\documentclass{article}
\usepackage{amsmath}

\begin{document}

\section*{Equality Conditions for Positive Real Variables}

Is the following equality true for all positive real numbers $x$ and $y$:
\begin{itemize}
    \item[a)] $(x + y)^2 = x^2 + 2xy + y^2$;
    \item[b)] $|x + y - 1| = |x + y| - 1$;
    \item[c)] $|x + y| = |x| + |y|$;
    \item[d)] $(x + y)^{-2} = x^{-2} + 2x^{-1}y^{-1} + y^{-2}$?
\end{itemize}

\section*{Solution}

\subsection*{a) $(x + y)^2 = x^2 + 2xy + y^2$}

This is true. From the definition of the square of a sum, we have:

\[
(x + y)^2 = x^2 + 2xy + y^2.
\]

\subsection*{b) $|x + y - 1| = |x + y| - 1$}

This equality doesn't always hold, especially when $x + y - 1 < 0$. For example, if $x = 0.5$ and $y = 0.3$, then:

\[
|x + y - 1| = |0.5 + 0.3 - 1| = |-0.2| = 0.2
\]
and
\[
|x + y| - 1 = |0.5 + 0.3| - 1 = 0.8 - 1 = -0.2.
\]

Thus, the equality doesn't hold.

\subsection*{c) $|x + y| = |x| + |y|$}

This equality holds only if both $x$ and $y$ are positive numbers. Therefore, for any positive real numbers $x$ and $y$, the equality holds:

\[
|x + y| = |x| + |y|.
\]

\subsection*{d) $(x + y)^{-2} = x^{-2} + 2x^{-1}y^{-1} + y^{-2}$}

This equation is false. We can provide a counterexample. Let $x = 1$ and $y = 2$. Letâ€™s calculate both sides of the equation.

Left-hand side:
\[
(x + y)^{-2} = (1 + 2)^{-2} = 3^{-2} = \frac{1}{9}.
\]

Right-hand side:
\[
x^{-2} + 2x^{-1}y^{-1} + y^{-2} = 1^{-2} + 2 \cdot 1^{-1} \cdot 2^{-1} + 2^{-2} = 1 + \frac{2}{2} + \frac{1}{4} = 1 + 1 + 0.25 = 2.25.
\]

We see that:

\[
\frac{1}{9} \neq 2.25.
\]

Thus, the equality does not hold.
\end{document}
